New and improved adom, incomplete proof

RelationalAlgebra/Equivalence/FOLtoRA/Adom.lean
@@ -5,11 +5,45 @@ open RM RA
 
 -- Utility for foldr
 @[simp]
-theorem RA.Query.foldr_join (xs : List α) (qb : α → RA.Query) (base : RA.Query) :
+theorem RA.Query.foldr_join_schema (xs : List α) (qb : α → RA.Query) (base : RA.Query) :
+  (xs.foldr (λ a q => q.j (qb a)) base).schema dbs = (xs.foldr (λ a s => s ∪ ((qb a).schema dbs))) (base.schema dbs) := by
+    induction xs
+    . simp
+    . simp_all
+
+@[simp]
+theorem RA.Query.foldr_join_evalT (xs : List α) (qb : α → RA.Query) (base : RA.Query) :
   (xs.foldr (λ a q => q.j (qb a)) base).evaluateT dbi = (xs.foldr (λ a s => joinT s ((qb a).evaluateT dbi))) (base.evaluateT dbi) := by
     induction xs
     . simp
     . simp_all
+
+@[simp]
+theorem RA.Query.foldr_union_evalT (xs : List α) (qb : α → RA.Query) (base : RA.Query) :
+  (xs.foldr (λ a q => q.u (qb a)) base).evaluateT dbi = {t | t ∈ base.evaluateT dbi ∨ ∃x ∈ xs, t ∈ (qb x).evaluateT dbi} := by
+    induction xs with
+    | nil =>
+      simp_all [List.foldr_nil, List.not_mem_nil, false_and]
+    | cons hd tl ih =>
+      simp_all only [List.foldr_cons, evaluateT.eq_6, unionT, List.mem_cons, exists_eq_or_imp]
+      ext x : 1
+      simp_all only [Set.mem_union, Set.mem_setOf_eq]
+      apply Iff.intro
+      · intro a
+        cases a with
+        | inl h =>
+          cases h with
+          | inl h_1 => simp_all only [true_or]
+          | inr h_2 => simp_all only [or_true]
+        | inr h_1 => simp_all only [true_or, or_true]
+      · intro a
+        cases a with
+        | inl h => simp_all only [true_or]
+        | inr h_1 =>
+          cases h_1 with
+          | inl h => simp_all only [or_true]
+          | inr h_2 => simp_all only [or_true, true_or]
+
 
 -- Database instance value domain
 def RM.DatabaseInstance.domain (dbi : DatabaseInstance) : Set Value :=
@@ -21,145 +55,395 @@ def adomRs (dbs : DatabaseSchema) : Set RelationName :=
 def adomAtts (dbs : DatabaseSchema) : Set Attribute :=
   {a | ∃rn, a ∈ dbs rn}
 
-def renameColumn (rn : RelationName) (a a' : Attribute) : RA.Query :=
-  (.p {a} (.r (renameFunc a a') (.R rn)))
 
-@[simp]
-theorem renameColumn.schema_def : (renameColumn rn a a').schema dbs = {a} := by
-  simp [renameColumn]
 
-@[simp]
-theorem renameColumn.isWellTyped_def (h'' : a' ∈ dbs rn) : (renameColumn rn a a').isWellTyped dbs := by
-  simp [renameColumn]
-  apply And.intro
-  . exact rename_func_bijective a a'
-  . use a'
-    simp_all [renameFunc]
+def RelationAttributeToColumn (rn : RelationName) (ra a : Attribute) : RA.Query :=
+  .r (renameFunc ra a) (.p {ra} (.R rn))
 
-@[simp]
-theorem renameColumn.evaluateT_def : (renameColumn rn a a').evaluateT dbi =
-  projectionT (renameT (dbi.relations rn).tuples (renameFunc a a')) {a} := by
-    simp [renameColumn]
+theorem RelationAttributeToColumn.schema_def : (RelationAttributeToColumn rn ra a).schema dbs = {a} := by
+  simp [RelationAttributeToColumn, renameFunc]
 
-def getColumn (rn : RelationName) (a : Attribute) (as : List Attribute) : RA.Query :=
-  as.foldr (λ a' q => q.u (renameColumn rn a a')) (.p {a} (Query.empty rn))
+theorem RelationAttributeToColumn.isWellTyped_def (h : ra ∈ dbs rn) :
+  (RelationAttributeToColumn rn ra a).isWellTyped dbs := by
+    simp [RelationAttributeToColumn, h, rename_func_bijective]
 
-@[simp]
-theorem getColumn.schema_def : (getColumn rn a as).schema dbs = {a} := by
+theorem RelationAttributeToColumn.evaluateT_def : (RelationAttributeToColumn rn ra a).evaluateT dbi =
+  {t | t ∈ (renameT (projectionT (dbi.relations rn).tuples {ra}) (renameFunc ra a))} := by
+    simp [RelationAttributeToColumn]
+
+theorem RelationAttributeToColumn.evalT_def (h_schema : ra ∈ dbi.schema rn) : (RelationAttributeToColumn rn ra a).evaluateT dbi =
+  {t | ∃t' ∈ (dbi.relations rn).tuples, t' ra = t a ∧ t.Dom = {a}} := by
+    ext t
+    simp [RelationAttributeToColumn]
+    simp_all only
+    apply Iff.intro
+    · intro a_1
+      obtain ⟨w, h⟩ := a_1
+      obtain ⟨left, right⟩ := h
+      use w
+      apply And.intro left
+      apply And.intro
+      . simp_all [renameFunc]
+      . have w_Dom : w.Dom = dbi.schema rn := by rw [← DatabaseInstance.validSchema,  RelationInstance.dom_eq_schema]; exact left
+        rw [← Finset.mem_coe, ← w_Dom] at h_schema
+        ext x
+        rw [Set.mem_singleton_iff, PFun.mem_dom]
+        simp [renameFunc] at right
+        by_cases hc : x = a
+        . simp_all [← PFun.mem_dom]
+        . by_cases hc' : x = ra
+          . subst hc'
+            have := (right a).2 (fun a_1 ↦ hc (id (Eq.symm a_1)))
+            simp_all
+          . have := (right x).2 hc'
+            simp_all
+    · intro a_1
+      obtain ⟨w, h⟩ := a_1
+      obtain ⟨left, right⟩ := h
+      simp_all only [ite_self, ↓reduceIte, renameFunc]
+      use w
+      apply And.intro left
+      intro a
+      apply And.intro
+      . exact fun h => right.1.symm
+      . intro h
+        obtain ⟨right_1, right_2⟩ := right
+        split
+        next h' =>
+          rw [Part.eq_none_iff', Part.dom_iff_mem, ← PFun.mem_dom, right_2]
+          rw [h'] at h
+          exact Set.notMem_singleton_iff.mpr fun a ↦ h (id (Eq.symm a))
+        next h =>
+          rw [Part.eq_none_iff', Part.dom_iff_mem, ← PFun.mem_dom, right_2]
+          simp [h]
+
+
+def RelationAttributesToColumn (rn : RelationName) (ras : List Attribute) (a : Attribute) (baseRa : Attribute) : RA.Query :=
+  ras.foldr (λ ra sq => .u sq ((RelationAttributeToColumn rn ra a))) (RelationAttributeToColumn rn baseRa a)
+
+theorem RelationAttributesToColumn.schema_def : (RelationAttributesToColumn rn ras a baseRa).schema dbs = {a} := by
+  simp [RelationAttributesToColumn]
+  induction ras with
+  | nil => simp [List.foldr_nil, RelationAttributeToColumn.schema_def]
+  | cons hd tl ih => simp_all only [List.foldr_cons, Query.schema.eq_6]
+
+theorem RelationAttributesToColumn.isWellTyped_def (h : baseRa ∈ dbs rn) (h' : ∀ra, ra ∈ ras → ra ∈ (dbs rn)) :
+  (RelationAttributesToColumn rn ras a baseRa).isWellTyped dbs := by
+    simp [RelationAttributesToColumn]
+    induction ras with
+    | nil => simp_all [List.foldr_nil, RelationAttributeToColumn.isWellTyped_def]
+    | cons hd tl ih =>
+      simp_all only [List.mem_cons, List.foldr_cons, Query.isWellTyped.eq_6, Query.isWellTyped]
+      apply And.intro
+      · apply ih
+        intro ra a_1
+        simp_all only [or_true, implies_true, forall_const, forall_eq_or_imp]
+      · apply And.intro
+        · apply RelationAttributeToColumn.isWellTyped_def (by simp_all)
+        · rw [← RelationAttributesToColumn];
+          simp_all [schema_def, RelationAttributeToColumn.schema_def]
+
+
+theorem RelationAttributesToColumn.evaluateT_def : (RelationAttributesToColumn rn ras a bRa).evaluateT dbi =
+  {t | t ∈ (RelationAttributeToColumn rn bRa a).evaluateT dbi ∨
+    (∃ra ∈ ras, t ∈ (RelationAttributeToColumn rn ra a).evaluateT dbi)
+  } := by
+    simp only [RelationAttributesToColumn, Query.foldr_union_evalT]
+
+theorem RelationAttributesToColumn.evalT_def (h_schema : ∀ra ∈ ras, ra ∈ dbi.schema rn) (h_schema' : bRa ∈ dbi.schema rn) : (RelationAttributesToColumn rn ras a bRa).evaluateT dbi =
+  {t | ∃t' ∈ (dbi.relations rn).tuples, (t' bRa = t a ∨ (∃ra ∈ ras, t' ra = t a)) ∧ t.Dom = {a}} := by
+    ext t
+    simp [RelationAttributesToColumn]
+    rw [RelationAttributeToColumn.evalT_def h_schema']
+    rw [Set.mem_setOf_eq]
+    simp only [or_and_right]
+    nth_rewrite 3 [← @bex_def]
+    simp only [exists_or]
+    apply or_congr
+    . apply exists_congr
+      simp [and_comm, and_assoc]
+    . simp only [exists_prop]
+      apply Iff.intro
+      . intro ⟨ra, hra, ht⟩
+        simp [RelationAttributeToColumn.evalT_def (h_schema ra hra)] at ht
+        obtain ⟨t', ht', ht'', ht'''⟩ := ht
+        use t'
+        apply And.intro ht' (And.intro ?_ ht''')
+        . use ra
+      . intro ⟨t', ht', ⟨ra, hra, hra'⟩, ht'''⟩
+        use ra
+        apply And.intro hra
+        simp [RelationAttributeToColumn.evalT_def (h_schema ra hra)]
+        use t'
+
+
+noncomputable def RelationNameToColumn (dbs : DatabaseSchema) (rn : RelationName) (a : Attribute) : RA.Query :=
+  RelationAttributesToColumn rn (dbs rn).ordering a ((dbs rn).ordering.headD (Classical.arbitrary Attribute))
+
+theorem RelationNameToColumn.schema_def :
+  (RelationNameToColumn dbs rn a).schema dbs = {a} := by
+    simp [RelationNameToColumn]
+    exact RelationAttributesToColumn.schema_def
+
+theorem RelationNameToColumn.isWellTyped_def (h : dbs rn ≠ ∅) :
+  (RelationNameToColumn dbs rn a).isWellTyped dbs := by
+    simp [RelationNameToColumn]
+    apply RelationAttributesToColumn.isWellTyped_def
+    . exact RelationSchema.ordering_head?_self_notEmpty h
+    . exact fun ra a ↦ (fun a rs ↦ (RelationSchema.ordering_mem a rs).mp) ra (dbs rn) a
+
+theorem RelationNameToColumn.evaluateT_def : (RelationNameToColumn dbs rn a).evaluateT dbi =
+  {t | (t ∈ ((RelationAttributesToColumn rn (dbs rn).ordering a ((dbs rn).ordering.headD (Classical.arbitrary Attribute))).evaluateT dbi))} := by
+    simp [RelationNameToColumn]
+
+theorem RelationNameToColumn.evalT_def (h : dbi.schema rn ≠ ∅) : (RelationNameToColumn dbi.schema rn a).evaluateT dbi =
+  {t | ∃t' ∈ (dbi.relations rn).tuples, (∃ra ∈ (dbi.schema rn), t' ra = t a) ∧ t.Dom = {a}} := by
+    rw [RelationNameToColumn, RelationAttributesToColumn.evalT_def]
+    . ext t
+      simp_all only [ne_eq, RelationSchema.ordering_mem, Set.mem_setOf_eq]
+      apply Iff.intro
+      · intro a_1
+        obtain ⟨w, h_1⟩ := a_1
+        obtain ⟨left, right⟩ := h_1
+        obtain ⟨left_1, right⟩ := right
+        simp_all only [and_true]
+        cases left_1 with
+        | inl h_1 =>
+          use w
+          simp_all only [true_and]
+          use ((dbi.schema rn).ordering.head?.getD (Classical.arbitrary Attribute))
+          simp_all
+        | inr h_2 =>
+          obtain ⟨w_1, h_1⟩ := h_2
+          obtain ⟨left_1, right_1⟩ := h_1
+          use w
+          simp_all only [true_and]
+          use w_1
+      · intro a_1
+        obtain ⟨w, h_1⟩ := a_1
+        obtain ⟨left, right⟩ := h_1
+        obtain ⟨left_1, right⟩ := right
+        obtain ⟨w_1, h_1⟩ := left_1
+        obtain ⟨left_1, right_1⟩ := h_1
+        simp_all only [and_true]
+        use w
+        simp_all only [true_and]
+        apply Or.inr
+        use w_1
+    . simp_all
+    . simp_all
+
+
+noncomputable def RelationNameToColumns (dbs : DatabaseSchema) (rn : RelationName) (as : List Attribute) : RA.Query :=
+  as.foldr (λ a sq => .j sq (RelationNameToColumn dbs rn a)) (.p ∅ (Query.empty rn))
+
+theorem RelationNameToColumns.schema_def : (RelationNameToColumns dbs rn as).schema dbs = as.toFinset := by
+  simp [RelationNameToColumns]
   induction as with
-  | nil => simp [getColumn]
-  | cons hd tl ih => simp_all [getColumn]
+  | nil => simp
+  | cons hd tl ih => simp_all [RelationNameToColumn.schema_def]
 
-@[simp]
-theorem getColumn.isWellTyped_def (h : a ∈ dbs rn) (h'' : ∀a', a' ∈ as → a' ∈ dbs rn) : (getColumn rn a as).isWellTyped dbs := by
-  induction as with
-  | nil => simp [getColumn, h, Query.empty]
-  | cons hd tl ih =>
-    simp_all [getColumn]
-    exact schema_def
-
-@[simp]
-theorem getColumn.evaluateT_def : (getColumn rn a as).evaluateT dbi =
-  {t | ∃a' ∈ as, t ∈ (renameColumn rn a a').evaluateT dbi} := by
+theorem RelationNameToColumns.isWellTyped_def (h : dbs rn ≠ ∅) :
+  (RelationNameToColumns dbs rn as).isWellTyped dbs := by
+    simp [RelationNameToColumns]
     induction as with
-    | nil =>
-      simp [getColumn, projectionT, Query.evaluateT.empty_def]
+    | nil => simp [List.foldr_nil]
     | cons hd tl ih =>
-      simp [getColumn, unionT]
-      rw [← getColumn, ih]
-      aesop
+      simp_all only [List.foldr_cons, Query.isWellTyped.eq_4, true_and, RelationNameToColumn.isWellTyped_def h]
 
-def joinColumns (rn : RelationName) (as as' : List Attribute) : RA.Query :=
-  as.foldr (λ a q => q.j (getColumn rn a as')) (.p {} (Query.empty rn))
-
-@[simp]
-theorem joinColumns.schema_def : (joinColumns rn as as').schema dbs = as.toFinset := by
-  induction as with
-  | nil => simp [joinColumns]
-  | cons hd tl ih => simp_all [joinColumns]
-
-@[simp]
-theorem joinColumns.isWellTyped_def {as as' : List Attribute} (h : ∀a', a' ∈ as → a' ∈ dbs rn) (h' : ∀a', a' ∈ as' → a' ∈ dbs rn) : (joinColumns rn as as').isWellTyped dbs := by
-  induction as with
-  | nil => simp [joinColumns, Query.empty]
-  | cons hd tl ih =>
-    simp [joinColumns]
-    simp_all
-    exact ih
-
-@[simp]
-theorem joinColumns.evaluateT_def : (joinColumns rn as as').evaluateT dbi =
-  (as.foldr (λ a s => joinT s ((getColumn rn a as').evaluateT dbi))) ((Query.empty rn).evaluateT dbi) := by
+theorem RelationNameToColumns.evaluateT_def : (RelationNameToColumns dbs rn as).evaluateT dbi =
+  (as.foldr (λ a s => joinT s ((RelationNameToColumn dbs rn a).evaluateT dbi))) ∅ := by
+    simp only [RelationNameToColumns]
     induction as with
-    | nil =>
-      simp [joinColumns, Query.evaluateT.empty_def, projectionT]
-    | cons hd tl ih =>
-      simp [joinColumns, Query.evaluateT.empty_def, projectionT]
+    | nil => simp
+    | cons hd tl ih => simp_all only [Query.foldr_join_evalT, joinT, RelationNameToColumn.evaluateT_def,
+        List.headD_eq_head?_getD, Set.setOf_mem_eq, PFun.mem_dom, forall_exists_index, Set.mem_union, not_or,
+        not_exists, and_imp, Query.evaluateT, projectionT, Query.evaluateT.empty_def, Set.mem_empty_iff_false,
+        Finset.notMem_empty, IsEmpty.forall_iff, not_false_eq_true, forall_const, true_and, false_and, exists_const,
+        Set.setOf_false, List.foldr_cons, Query.evaluateT.eq_4]
 
-def unionRels (rns : List RelationName) (as : List Attribute) : RA.Query :=
-  rns.foldr (λ rn q => q.u (joinColumns rn as as)) (.p as.toFinset (Query.empty default))
-
-theorem unionRels_def (rns) (as) : unionRels rns as = rns.foldr (λ rn q => q.u (joinColumns rn as as)) (.p as.toFinset (Query.empty default)) := by rfl
-
-@[simp]
-theorem unionRels.schema_def : (unionRels rns as).schema dbs = as.toFinset := by
-  induction rns with
-  | nil => simp [unionRels]
-  | cons hd tl ih => simp_all [unionRels]
-
-@[simp]
-theorem unionRels.isWellTyped_def {as : List Attribute} (h : ∀rn, ∀a', a' ∈ as → a' ∈ dbs rn) : (unionRels rns as).isWellTyped dbs := by
-  induction rns with
-  | nil => simp [unionRels, Finset.subset_iff, Query.empty]; exact h ""
-  | cons hd tl ih =>
-    simp [unionRels]
-    apply And.intro
-    · exact ih
-    · apply And.intro
-      . exact joinColumns.isWellTyped_def (h hd) (h hd)
-      . rw [← String.default_eq, ← unionRels_def tl as]
-        exact schema_def
-
-@[simp]
-theorem unionRels.evaluateT_def : (unionRels rns as).evaluateT dbi =
-  {t | ∃rn ∈ rns, t ∈ (joinColumns rn as as).evaluateT dbi} := by
-    induction rns with
-    | nil =>
-      simp [unionRels, projectionT, Query.evaluateT.empty_def]
-    | cons hd tl ih =>
-      simp [unionRels, unionT]
-      rw [← String.default_eq, ← unionRels, ih]
-      ext x : 1
-      simp_all only [joinColumns.evaluateT_def, joinT, getColumn.evaluateT_def,
-        renameColumn.evaluateT_def, projectionT, renameT, exists_eq_right', Set.mem_setOf_eq,
-        Finset.mem_singleton, PFun.mem_dom, forall_exists_index, Set.mem_union, not_or, not_exists,
-        and_imp, Query.evaluateT.empty_def]
-      apply Iff.intro Or.symm Or.symm
-
-variable (dbs : DatabaseSchema) [hf : Fintype ↑(adomRs dbs)]
-
-def adom (rs : RelationSchema) : Query :=
-  unionRels ((adomRs dbs).toFinset.sort (.≤.)) rs.ordering
-
-@[simp]
-theorem adom_schema : ↑((adom dbs rs).schema dbs) = rs := by
-  ext a
-  simp [adom]
-
-@[simp]
-theorem adom.isWellTyped_def (h : ↑rs ⊆ adomAtts dbs) : (adom dbs rs).isWellTyped dbs := by
-  simp [adom]; exact unionRels.isWellTyped_def (by simp_all [adomAtts]; intro rn a ha; sorry)
-
-@[simp]
-theorem adom.evaluateT_def (dbi : DatabaseInstance) : (adom dbs rs).evaluateT dbi =
-  (unionRels
-    ((adomRs (dbs)).toFinset.sort (.≤.))
-    (rs.ordering)
-  ).evaluateT dbi :=
-    by rfl
-
--- main theorem
-theorem adom_all {dbi : DatabaseInstance} (h_attr : a ∈ rs) (h_val : v ∈ dbi.domain) (h_wt : (adom dbs rs).isWellTyped dbs) :
-  ∃ t ∈ (adom dbs rs).evaluateT dbi, t a = v := by
-    simp_all [DatabaseInstance.domain, adomRs, adom]
+theorem RelationNameToColumns.evalT_def (h : dbi.schema rn ≠ ∅) : (RelationNameToColumns dbi.schema rn as).evaluateT dbi =
+  {t | t.Dom = as.toFinset.toSet ∧ ∃a ∈ as, ∃ra ∈ (dbi.schema rn), ∃t' ∈ (dbi.relations rn).tuples, (t' ra = t a)} := by
     sorry
+
+noncomputable def RelationNamesToColumns (dbs : DatabaseSchema) (rns : List RelationName) (as : List Attribute) (baseRn : RelationName) : RA.Query :=
+  rns.foldr (λ rn sq => .u sq (RelationNameToColumns dbs rn as)) (RelationNameToColumns dbs baseRn as)
+
+theorem RelationNamesToColumns.schema_def: (RelationNamesToColumns dbs rns as baseRn).schema dbs = as.toFinset := by
+  simp [RelationNamesToColumns]
+  induction rns with
+  | nil => simp [RelationNameToColumns.schema_def]
+  | cons hd tl ih => simp_all only [List.foldr_cons, Query.schema.eq_6]
+
+theorem RelationNamesToColumns.isWellTyped_def (h : dbs baseRn ≠ ∅) (h' : ∀rn ∈ rns, dbs rn ≠ ∅) :
+    (RelationNamesToColumns dbs rns as baseRn).isWellTyped dbs := by
+      simp [RelationNamesToColumns]
+      induction rns with
+      | nil => simp only [List.foldr_nil, RelationNameToColumns.isWellTyped_def h]
+      | cons hd tl ih =>
+        simp_all only [List.foldr_cons, Query.isWellTyped.eq_6]
+        simp_all only [ne_eq, List.mem_cons, or_true, not_false_eq_true, implies_true, forall_const, forall_eq_or_imp,
+          true_and]
+        obtain ⟨left, right⟩ := h'
+        apply And.intro
+        · apply RelationNameToColumns.isWellTyped_def left
+        · rw [← RelationNamesToColumns]
+          rw [schema_def]
+          rw [RelationNameToColumns.schema_def]
+
+theorem RelationNamesToColumns.evaluateT_def : (RelationNamesToColumns dbs rns as baseRn).evaluateT dbi =
+  {t | t ∈ ((RelationNameToColumns dbs baseRn as).evaluateT dbi) ∨ (∃rn ∈ rns, t ∈ ((RelationNameToColumns dbs rn as).evaluateT dbi)) } := by
+      simp only [RelationNamesToColumns, Query.foldr_union_evalT]
+
+theorem RelationNamesToColumns.evalT_def  (h : dbi.schema baseRn ≠ ∅) (h' : ∀rn ∈ rns, dbi.schema rn ≠ ∅) : (RelationNamesToColumns dbi.schema rns as baseRn).evaluateT dbi =
+  {t | ∃rn, (rn = baseRn ∨ rn ∈ rns) ∧ t.Dom = as.toFinset.toSet ∧ ∃a ∈ as, ∃ra ∈ (dbi.schema rn), ∃t' ∈ (dbi.relations rn).tuples, (t' ra = t a)} := by
+    ext t
+    rw [RelationNamesToColumns.evaluateT_def]
+    simp
+    apply or_congr
+    . rw [RelationNameToColumns.evalT_def h]
+      simp
+    . apply exists_congr
+      intro rn
+      apply Iff.intro
+      . intro h''
+        rw [RelationNameToColumns.evalT_def] at h''
+        . simp_all
+        . exact h' rn h''.1
+      . intro h''
+        rw [RelationNameToColumns.evalT_def]
+        . simp_all
+        . exact h' rn h''.1
+
+
+noncomputable def adom (dbs : DatabaseSchema) (rs : RelationSchema) [Fintype ↑(adomRs dbs)] : RA.Query :=
+  RelationNamesToColumns dbs (adomRs dbs).toFinset.toList rs.ordering ((adomRs dbs).toFinset.toList.headD (Classical.arbitrary RelationName))
+
+theorem adom.schema_def [Fintype ↑(adomRs dbs)] : (adom dbs rs).schema dbs = rs := by
+  simp [adom, RelationNamesToColumns.schema_def]
+
+theorem adom.isWellTyped_def[Fintype ↑(adomRs dbs)] [ne : Nonempty (adomRs dbs)] :
+    (adom dbs rs).isWellTyped dbs := by
+      simp [adom]
+      refine RelationNamesToColumns.isWellTyped_def ?_ ?_
+      . simp at ne
+        simp
+        simp_all [Option.getD]
+        split
+        next opt x heq =>
+          simp [List.head?_eq_some_iff] at heq
+          obtain ⟨w, h_1⟩ := heq
+          have : x ∈ (adomRs dbs).toFinset.toList := by simp_all
+          have : x ∈ (adomRs dbs) := by simp at this; exact this
+          rw [adomRs] at this
+          exact this
+        next opt heq =>
+          simp_all [List.head?_eq_none_iff]
+      . intro rn a
+        simp_all only [Finset.mem_toList, Set.mem_toFinset, ne_eq]
+        exact a
+
+theorem adom.evaluateT_def [Fintype ↑(adomRs dbs)] : (adom dbs as).evaluateT dbi =
+  {t | t ∈ ((RelationNameToColumns dbs ((adomRs dbs).toFinset.toList.headD (Classical.arbitrary RelationName)) as.ordering).evaluateT dbi)
+    ∨ (∃rn ∈ (adomRs dbs).toFinset.toList, t ∈ ((RelationNameToColumns dbs rn as.ordering).evaluateT dbi)) } := by
+      rw [adom, ← @RelationNamesToColumns.evaluateT_def]
+
+@[simp]
+theorem adom.complete_def [Fintype ↑(adomRs dbi.schema)] [ne : Nonempty (adomRs dbi.schema)] : (adom dbi.schema as).evaluateT dbi =
+  {t | t.Dom = ↑as ∧ ∃a ∈ as, ∃v ∈ dbi.domain, t a = .some v} := by
+    rw [adom, RelationNamesToColumns.evalT_def]
+    . rw [DatabaseInstance.domain]
+      ext t
+      simp_all only [nonempty_subtype, List.headD_eq_head?_getD, Finset.mem_toList, Set.mem_toFinset,
+        RelationSchema.ordering_eq_toFinset, RelationSchema.ordering_mem, exists_eq_or_imp, Set.mem_setOf_eq,
+        Set.mem_image]
+      obtain ⟨w, h⟩ := ne
+      apply Iff.intro
+      · intro a
+        cases a with
+        | inl h_1 =>
+          obtain ⟨left, right⟩ := h_1
+          obtain ⟨w_1, h_1⟩ := right
+          obtain ⟨left_1, right⟩ := h_1
+          obtain ⟨w_2, h_1⟩ := right
+          obtain ⟨left_2, right⟩ := h_1
+          obtain ⟨w_3, h_1⟩ := right
+          obtain ⟨left_3, right⟩ := h_1
+          apply And.intro left
+          use w_1
+          apply And.intro left_1
+          have : (t w_1).Dom := by
+            rw [← right, Part.dom_iff_mem, ← PFun.mem_dom]
+            rw [(dbi.relations _).validSchema w_3 left_3, Finset.mem_coe, DatabaseInstance.validSchema]
+            exact left_2
+          use (t w_1).get this
+          simp_all only [Part.some_get, and_true]
+          apply Exists.intro
+          · apply Exists.intro
+            · apply Exists.intro
+              · apply And.intro
+                · exact left_3
+                · exact right
+        | inr h_2 =>
+          obtain ⟨w_1, h_1⟩ := h_2
+          obtain ⟨left, right⟩ := h_1
+          obtain ⟨left_1, right⟩ := right
+          obtain ⟨w_2, h_1⟩ := right
+          obtain ⟨left_2, right⟩ := h_1
+          obtain ⟨w_3, h_1⟩ := right
+          obtain ⟨left_3, right⟩ := h_1
+          obtain ⟨w_4, h_1⟩ := right
+          obtain ⟨left_4, right⟩ := h_1
+          apply And.intro left_1
+          use w_2
+          apply And.intro left_2
+          have : (t w_2).Dom := by
+            rw [← right, Part.dom_iff_mem, ← PFun.mem_dom]
+            rw [(dbi.relations w_1).validSchema w_4 left_4, Finset.mem_coe, DatabaseInstance.validSchema]
+            exact left_3
+          use (t w_2).get this
+          simp_all only [Part.some_get, and_true]
+          apply Exists.intro
+          · apply Exists.intro
+            · apply Exists.intro
+              · apply And.intro
+                · exact left_4
+                · exact right
+      · intro a
+        simp_all only [true_and]
+        obtain ⟨left, right⟩ := a
+        obtain ⟨a, h_1⟩ := right
+        obtain ⟨left_1, right⟩ := h_1
+        obtain ⟨v, h_1⟩ := right
+        obtain ⟨left_2, right⟩ := h_1
+        obtain ⟨rn', h_1⟩ := left_2
+        obtain ⟨ra, h_1⟩ := h_1
+        obtain ⟨t', h_1⟩ := h_1
+        obtain ⟨ht', ht'_eq⟩ := h_1
+        apply Or.inr
+        use rn'
+        have : ra ∈ dbi.schema rn' := by
+          have := (dbi.relations rn').validSchema t' ht'
+          simp only [Set.ext_iff, PFun.mem_dom, DatabaseInstance.validSchema, Finset.mem_coe] at this
+          exact (this ra).mp (Exists.intro v (Part.eq_some_iff.mp ht'_eq))
+        apply And.intro
+        . rw [adomRs, Set.mem_setOf_eq]
+          by_contra hc
+          rw [hc] at this
+          exact (Finset.notMem_empty ra) this
+        . use a
+          simp [left_1]
+          use ra
+          apply And.intro this
+          . use t'
+            simp_all
+
+    . simp_all [Option.getD]
+      split
+      next opt rn' heq =>
+        simp_all [List.head?_eq_some_iff]
+        obtain ⟨w_1, h_1⟩ := heq
+        have : rn' ∈ adomRs dbi.schema := by rw [← Set.mem_toFinset, ← Finset.mem_toList]; simp only [h_1, List.mem_cons, true_or]
+        simp_all [adomRs]
+      next opt heq => simp_all [Set.ext_iff]
+    . simp_all [adomRs]
